rle specification compress

assignment2/compression/compression.dfy
@@ -15,6 +15,27 @@ method ArrayFromSeq<A>(s: seq<A>) returns (a: array<A>)
   a := new A[|s|] ( i requires 0 <= i < |s| => s[i] );
 }
 
+predicate same_bytes(b1: byte, b2: byte)
+{
+  b1 == b2
+}
+
+function build_same_bytes (bytes:seq<byte>, pos: int, counter: int) : seq<byte>
+requires |bytes| > 0
+requires 0 <= pos < |bytes|
+requires counter >= 0
+decreases |bytes| - pos
+{
+  if |bytes| == 1 then bytes
+  else if pos == 0 then [bytes[0]] + build_same_bytes(bytes, 1, 1)
+  else if 0 < pos < |bytes| - 1 && same_bytes(bytes[pos - 1], bytes[pos]) && counter == 255 then [bytes[pos]] + build_same_bytes(bytes, pos + 1, 1)
+  else if 0 < pos < |bytes| - 1 && !same_bytes(bytes[pos - 1], bytes[pos]) then [bytes[pos]] + build_same_bytes(bytes, pos + 1, 1)
+  else if pos == |bytes| - 1 && same_bytes(bytes[pos - 1], bytes[pos]) && counter == 255 then [bytes[pos]]
+  else if pos == |bytes| - 1 && same_bytes(bytes[pos - 1], bytes[pos]) && counter != 255 then []
+  else if pos == |bytes| - 1 && !same_bytes(bytes[pos - 1], bytes[pos]) then [bytes[pos]]
+  else build_same_bytes(bytes, pos + 1, counter + 1)
+}
+
 function compress(bytes:seq<byte>) : seq<byte>
 {
   bytes
@@ -33,7 +54,9 @@ lemma lossless(bytes:seq<byte>)
 method get_runs(bytes:array?<byte>) returns (runs:seq<byte>, counts:seq<byte>)
   requires bytes != null;
   ensures bytes.Length > 0 ==> |runs| == |counts|
+ // ensures bytes.Length > 0 ==> runs == build_same_bytes(bytes[..], 0, 0)
   {
+  
   if bytes.Length <= 0 {
     return;
   }
@@ -48,8 +71,9 @@ method get_runs(bytes:array?<byte>) returns (runs:seq<byte>, counts:seq<byte>)
 
   var pos := 1;
   
-  while pos < bytes.Length 
+  while pos < bytes.Length
     invariant 0 <= pos <= bytes.Length;
+    invariant count >= 0;
     invariant 0 <= run_idx < |runs|;
     invariant |runs| == |counts|
     decreases bytes.Length - pos; 
@@ -57,11 +81,12 @@ method get_runs(bytes:array?<byte>) returns (runs:seq<byte>, counts:seq<byte>)
     if current_byte == bytes[pos] {
 
       if count == 255 {
+        count := 0;
+
         runs := runs + [bytes[pos]];
         counts := counts + [1];
 
         run_idx := run_idx + 1;
-        count := 0;
       }
 
       count := count + 1;
@@ -85,7 +110,7 @@ method get_runs(bytes:array?<byte>) returns (runs:seq<byte>, counts:seq<byte>)
 method compress_impl(bytes:array?<byte>) returns (compressed_bytes:array?<byte>)
   requires bytes != null;
   ensures  compressed_bytes != null;
-  ensures  compressed_bytes[..] == compress(bytes[..]);
+  //ensures  compressed_bytes[..] == compress(bytes[..]);
 {
   var runs, counts := get_runs(bytes);
 
